all clean now, and deconstrucitno paper is up to date

Abstraction_calculus/Abstraction_Equal.v.d
@@ -1,0 +1,2 @@
+Abstraction_Equal.vo Abstraction_Equal.glob Abstraction_Equal.v.beautified: Abstraction_Equal.v
+Abstraction_Equal.vio: Abstraction_Equal.v
