Abstraction_calculus/Abstraction_Normal.v.d
@@ -1,0 +1,2 @@
+Abstraction_Normal.vo Abstraction_Normal.glob Abstraction_Normal.v.beautified: Abstraction_Normal.v
+Abstraction_Normal.vio: Abstraction_Normal.v
