Abstraction_calculus/Abstraction_Tactics.v.d
@@ -1,0 +1,2 @@
+Abstraction_Tactics.vo Abstraction_Tactics.glob Abstraction_Tactics.v.beautified: Abstraction_Tactics.v
+Abstraction_Tactics.vio: Abstraction_Tactics.v
