Abstraction_calculus/Abstraction_Terms.v.d
@@ -1,0 +1,2 @@
+Abstraction_Terms.vo Abstraction_Terms.glob Abstraction_Terms.v.beautified: Abstraction_Terms.v
+Abstraction_Terms.vio: Abstraction_Terms.v
