Abstraction_calculus/Closure_to_Abstraction.v.d
@@ -1,0 +1,2 @@
+Closure_to_Abstraction.vo Closure_to_Abstraction.glob Closure_to_Abstraction.v.beautified: Closure_to_Abstraction.v
+Closure_to_Abstraction.vio: Closure_to_Abstraction.v
