Abstraction_calculus/Closure_to_Abstraction.v
@@ -26,8 +26,8 @@
 Add LoadPath ".." as IntensionalLib.
 
 Require Import Arith.
-Require Import IntensionalLib.Closure_calculus.Closure_calculus. 
 Require Import IntensionalLib.SF_calculus.General.
+Require Import IntensionalLib.Closure_calculus.Closure_calculus. 
 Require Import IntensionalLib.Abstraction_calculus.Abstraction_Terms. 
 Require Import IntensionalLib.Abstraction_calculus.Abstraction_Tactics.
 Require Import IntensionalLib.Abstraction_calculus.Abstraction_Reduction.
@@ -64,18 +64,18 @@ Hint Resolve ref_normal var_ref_normal.
 
 
 
-Fixpoint l2SF (t: lambda) := 
+Fixpoint closure_to_abstraction (t: lambda) := 
 match t with 
 | Closure_calculus.Ref i => App (Op Var) (ref i)
-| Closure_calculus.Tag s t => App (App (Op Tag) (l2SF s)) (l2SF t)
-| Closure_calculus.App t u => App (l2SF t) (l2SF u) 
+| Closure_calculus.Tag s t => App (App (Op Tag) (closure_to_abstraction s)) (closure_to_abstraction t)
+| Closure_calculus.App t u => App (closure_to_abstraction t) (closure_to_abstraction u) 
 | Closure_calculus.Iop => Op Iop
-| Closure_calculus.Add sigma i u => App (App (App (Op Add) (l2SF sigma)) (ref i)) (l2SF u)
-| Closure_calculus.Abs sigma j t => App (App (App (Op Abs) (l2SF sigma)) (ref j)) (l2SF t)
+| Closure_calculus.Add sigma i u => App (App (App (Op Add) (closure_to_abstraction sigma)) (ref i)) (closure_to_abstraction u)
+| Closure_calculus.Abs sigma j t => App (App (App (Op Abs) (closure_to_abstraction sigma)) (ref j)) (closure_to_abstraction t)
 end.
 
 
-Lemma l2SF_preserves_red: forall M N, seq_red1 M N -> c_red (l2SF M) (l2SF N).
+Lemma closure_to_abstraction_preserves_red1: forall M N, seq_red1 M N -> c_red (closure_to_abstraction M) (closure_to_abstraction N).
 Proof.
 intros M N r; induction r; split_all. 
 (* 2 *)
@@ -87,6 +87,22 @@ eapply2 unequal_normal. intro. eapply2 H. eapply2 ref_monotonic. auto. auto.
 eapply2 succ_red.
 Qed.
 
-Lemma l2SF_preserves_normal : forall M, Closure_calculus.normal M -> normal (l2SF M). 
+
+Definition implies_red (red1 : lambda -> lambda -> Prop) (red2: termred) := 
+forall M N, red1 M N -> red2(closure_to_abstraction M) (closure_to_abstraction N). 
+
+Lemma implies_red_multi_step: forall red1 red2, implies_red red1  (multi_step red2) -> 
+                                                implies_red (Closure_calculus.multi_step red1) (multi_step red2).
+Proof. red. 
+intros red1 red2 IR M N R; induction R; split_all. 
+apply transitive_red with (closure_to_abstraction N); auto. 
+Qed. 
+
+Theorem closure_to_abstraction_preserves_reduction: forall M N, Closure_calculus.seq_red M N -> c_red (closure_to_abstraction M) (closure_to_abstraction N).
+Proof. intros. eapply2 (implies_red_multi_step). red. apply closure_to_abstraction_preserves_red1.
+Qed. 
+
+
+Theorem closure_to_abstraction_preserves_normal : forall M, Closure_calculus.normal M -> normal (closure_to_abstraction M). 
 Proof. intros M nf; induction nf; split_all.  Qed. 
 
